dice/src/l0/asn1/ASN1.Low.Length.fsti
@@ -17,6 +17,8 @@ open FStar.Integers
 
 // noextract inline_for_extraction unfold
 // [@@ "opaque_to_smt"]
+[@@ strict_on_arguments [0]]
+inline_for_extraction
 let len_of_asn1_length
   (len: asn1_int32)
 : (offset: U32.t {v offset == Seq.length (serialize serialize_asn1_length len)})
