dice/src/l0/asn1/ASN1.Low.Value.OID.fsti
@@ -8,6 +8,7 @@ open FStar.Integers
 
 // inline_for_extraction noextract unfold
 // [@@ "opaque_to_smt"]
+inline_for_extraction noextract
 let len_of_oid
   (oid: oid_t)
 : Tot (len: asn1_value_int32_of_type OID
